
\documentclass{article}

\usepackage{amsmath}
\usepackage{amsfonts}
\usepackage[utf8]{inputenc}
\usepackage[a4paper]{geometry}
\usepackage[shortlabels]{enumitem}
\usepackage{hyperref}

\makeatletter
\renewcommand{\@seccntformat}[1]{}
\makeatother

\makeatletter
\newcommand*{\rom}[1]{\expandafter\@slowromancap\romannumeral #1@}
\makeatother

\setlength\parindent{0pt}

\title{Analysis Übung 2}
\author{Ahmed Bajra}
\date{2020-09-25}

\begin{document}
    \maketitle

    \section{Übungen}
    8b)

    \begin{align*}
        a_n & =  \sum_{1\leq k\leq n}\frac{k}{n^2} \\
        & =  \frac{1}{n^2}\frac{n(n+1)}{2}\\
        & =  \frac12 + \frac1{2n}\\
        \lim_{n\rightarrow\infty}a_n & =  \frac12 \Rightarrow (\text{Konvergiert}) \\
        \\
        a_{n+1} = \frac12 + \frac{1}{2(n+1)} & <  a_n \Rightarrow  \text{Strikt monoton fallend}
    \end{align*}

    8d)

    \begin{align*}
        a_1&=0\\
        a_2&=1\\
        a_n&=\frac12(a_{n-1}+a_{n-2})\\
        a_{n+2}-a_{n+1} &= \frac12(a_{n+1}+a_n) - a_{n+1}\\
        &= \frac12(a_n - a_{n+1})\\
        &= -\frac12(a_{n+1} -a_n) \\
        &= \left(-\frac12\right)^2(a_{\underline{n}}-a_{n-1}) \\
        &= \left(-\frac12\right)^{n-k+2}(a_{k}-a_{k-1}) \\
        &= \left(-\frac12\right)^{n}(a_{2}-a_{1}) = \left(-\frac12\right)^{n} \\
    \end{align*}

    \newpage

    \begin{align*}
        a_{n+2}-a_{n+1} &= \left(-\frac12\right)^{n} \\
        a_n &= a_1 &+ (a_2 - a_1) &+ \dots &+ (a_{n-1} - a_{n-2}) &+ (a_n - a_{n-1})\\
        &= a_1 &+ 1 &+ \dots &+  \left(-\frac12\right)^{n-3} &+  \left(-\frac12\right)^{n-2}\\
        &= \sum_{0\leq k \leq n-2}\left(-\frac12\right)^{k} 
    \end{align*}

    9a) Fibonacci

    \begin{align*}
        a_n &:= a_{n-1} + a_{n-2} \\
        b_n &= \frac{a_n}{a_{n-1}} \\
        &= \frac{a_{n-1} + a_{n-2}}{a_{n-1}}\\
        &= 1 + \frac{a_{n-1}}{a_{n-2}} \\
        &= 1 + \frac1{b_{n-1}} \\
        b_1 &= 1 \leq b_n  \\
        1 + \frac1{b_{n-1}} &\leq 2 \\
        \Rightarrow & 1 \leq b_n \leq 2
    \end{align*}

    \newpage

    

\end{document}